Get the inferencer building and verified again

inference/inferScript.sml
@@ -4,6 +4,9 @@ open stringTheory monadsyntax;
 
 val _ = new_theory "infer";
 
+val list_subset_def = Define `
+list_subset l1 l2 = EVERY (\x. MEM x l2) l1`;
+
 (* 'a is the type of the state, 'b is the type of successful computations, and
  * 'c is the type of exceptions *)
 
@@ -433,7 +436,7 @@ val infer_e_def = tDefine "infer_e" `
  rw []);
 
 val infer_d_def = Define `
-(infer_d mn tdecs menv cenv env (Dlet p e) = 
+(infer_d mn decls menv cenv env (Dlet p e) = 
   do () <- init_state;
      n <- get_next_uvar;
      t1 <- infer_e menv cenv env e;
@@ -443,9 +446,9 @@ val infer_d_def = Define `
      ts <- apply_subst_list (MAP SND env');
      (num_tvs, s, ts') <- return (generalise_list n 0 FEMPTY ts);
      () <- guard (num_tvs = 0 ∨ is_value e) "Value restriction violated";
-     return (tdecs, [], ZIP (MAP FST env', MAP (\t. (num_tvs, t)) ts'))
+     return (([],[],[]), [], ZIP (MAP FST env', MAP (\t. (num_tvs, t)) ts'))
   od) ∧
-(infer_d mn tdecs menv cenv env (Dletrec funs) =
+(infer_d mn decls menv cenv env (Dletrec funs) =
   do () <- guard (ALL_DISTINCT (MAP FST funs)) "Duplicate function name";
      () <- init_state;
      next <- get_next_uvar;
@@ -455,27 +458,31 @@ val infer_d_def = Define `
      () <- add_constraints uvars funs_ts;
      ts <- apply_subst_list uvars;
      (num_gen,s,ts') <- return (generalise_list next 0 FEMPTY ts);
-     return (tdecs, [], list$MAP2 (\(f,x,e) t. (f,(num_gen,t))) funs ts')
+     return (([],[],[]), [], list$MAP2 (\(f,x,e) t. (f,(num_gen,t))) funs ts')
   od) ∧
-(infer_d mn tdecs menv cenv env (Dtype tdefs) =
-  if check_ctor_tenv mn cenv tdefs then
-    return (tdecs, build_ctor_tenv mn tdefs, [])
-  else
-    failwith "Bad type definition") ∧
-(infer_d mn tdecs menv cenv env (Dexn cn ts) =
-  if check_exn_tenv mn cenv cn ts then
-    return (tdecs, bind cn ([], ts, TypeExn (mk_id mn cn)) emp, [])
-  else
-    failwith "Bad type definition")`;
+(infer_d mn (mdecls,tdecls,edecls) menv cenv env (Dtype tdefs) =
+  do () <- guard (check_ctor_tenv mn tdefs) "Bad type definition";
+     new_tdecls <- return (MAP (\(tvs,tn,ctors). mk_id mn tn) tdefs);
+     () <- guard (EVERY (\new_id. ~MEM new_id tdecls) new_tdecls) "Duplicate type definition";
+     return (([],new_tdecls,[]), build_ctor_tenv mn tdefs, [])
+  od) ∧
+(infer_d mn (mdecls,tdecls,edecls) menv cenv env (Dexn cn ts) =
+  do () <- guard (check_exn_tenv mn cn ts) "Bad exception definition";
+     () <- guard (~MEM (mk_id mn cn) edecls) "Duplicate exception definition";
+     return (([],[],[mk_id mn cn]), bind cn ([], ts, TypeExn (mk_id mn cn)) emp, [])
+  od)`;
+
+val append_decls_def = Define `
+append_decls (m1,t1,e1) (m2,t2,e2) = (m1++m2,t1++t2,e1++e2)`;
 
 val infer_ds_def = Define `
-(infer_ds mn tdecs menv cenv env [] =
-  return (tdecs, [],[])) ∧
-(infer_ds mn tdecs menv cenv env (d::ds) =
+(infer_ds mn decls menv cenv env [] =
+  return (([],[],[]), [],[])) ∧
+(infer_ds mn decls menv cenv env (d::ds) =
   do
-    (tdecs',cenv',env') <- infer_d mn tdecs menv cenv env d;
-    (tdecs'',cenv'',env'') <- infer_ds mn tdecs' menv (merge_tenvC ([],cenv') cenv) (env' ++ env) ds;
-    return (tdecs'', merge cenv'' cenv', env'' ++ env')
+    (decls',cenv',env') <- infer_d mn decls menv cenv env d;
+    (decls'',cenv'',env'') <- infer_ds mn (append_decls decls' decls) menv (merge_tenvC ([],cenv') cenv) (env' ++ env) ds;
+    return (append_decls decls'' decls', merge cenv'' cenv', env'' ++ env')
   od)`;
 
 val t_to_freevars_def = Define `
@@ -493,25 +500,28 @@ val t_to_freevars_def = Define `
   od)`;
 
 val check_specs_def = Define `
-(check_specs mn cenv env [] =
-  return (cenv,env)) ∧
-(check_specs mn cenv env (Sval x t::specs) =
+(check_specs mn decls cenv env [] =
+  return (decls,cenv,env)) ∧
+(check_specs mn decls cenv env (Sval x t::specs) =
   do fvs <- t_to_freevars t;
      fvs' <- return (nub fvs);
-     check_specs mn cenv (bind x (LENGTH fvs', infer_type_subst (ZIP (fvs', MAP Infer_Tvar_db (COUNT_LIST (LENGTH fvs')))) t) env) specs
+     check_specs mn decls cenv (bind x (LENGTH fvs', infer_type_subst (ZIP (fvs', MAP Infer_Tvar_db (COUNT_LIST (LENGTH fvs')))) t) env) specs
   od) ∧
-(check_specs mn cenv env (Stype td :: specs) =
-  do () <- guard (check_ctor_tenv mn ((emp,cenv):tenvC) td) "Bad type definition";
-     check_specs mn (merge (build_ctor_tenv mn td) cenv) env specs
+(check_specs mn (mdecls,tdecls,edecls) cenv env (Stype tdefs :: specs) =
+  do () <- guard (check_ctor_tenv mn tdefs) "Bad type definition";
+     new_tdecls <- return (MAP (\(tvs,tn,ctors). mk_id mn tn) tdefs);
+     () <- guard (EVERY (\new_id. ~MEM new_id tdecls) new_tdecls) "Duplicate type definition";
+     check_specs mn (mdecls,new_tdecls++tdecls,edecls) (merge (build_ctor_tenv mn tdefs) cenv) env specs
   od) ∧
-(check_specs mn cenv env (Sexn cn ts :: specs) =
-  do () <- guard (check_exn_tenv mn ((emp,cenv):tenvC) cn ts) "Bad exception definition";
-     check_specs mn (bind cn ([], ts, TypeExn (mk_id mn cn)) cenv) env specs
+(check_specs mn (mdecls,tdecls,edecls) cenv env (Sexn cn ts :: specs) =
+  do () <- guard (check_exn_tenv mn cn ts) "Bad exception definition";
+     () <- guard (~MEM (mk_id mn cn) edecls) "Duplicate exception definition";
+     check_specs mn (mdecls,tdecls,mk_id mn cn::edecls) (bind cn ([], ts, TypeExn (mk_id mn cn)) cenv) env specs
   od) ∧
-(check_specs mn cenv env (Stype_opq tvs tn :: specs) =
-  do () <- guard (EVERY (\(cn,(x,y,tn')). TypeId (mk_id mn tn) ≠ tn') cenv) "Duplicate type definition";
+(check_specs mn (mdecls,tdecls,edecls) cenv env (Stype_opq tvs tn :: specs) =
+  do () <- guard (~MEM (mk_id mn tn) tdecls) "Duplicate type definition";
      () <- guard (ALL_DISTINCT tvs) "Duplicate type variables";
-     check_specs mn cenv env specs
+     check_specs mn (mdecls,mk_id mn tn::tdecls,edecls) cenv env specs
   od)`;
 
 val check_flat_weakC_def = Define `
@@ -538,38 +548,45 @@ val check_weakE_def = Define `
            check_weakE env_impl env_spec
         od)`;
 
+val check_weak_decls_def = Define `
+check_weak_decls (mdecls_impl,tdecls_impl,edecls_impl) (mdecls_spec,tdecls_spec,edecls_spec) ⇔
+  mdecls_spec = mdecls_impl ∧
+  list_subset tdecls_spec tdecls_impl ∧
+  list_subset edecls_spec edecls_impl`;
+
 val check_signature_def = Define `
-(check_signature mn cenv env NONE = 
-  return (cenv, env)) ∧
-(check_signature mn cenv env (SOME specs) =
-  do (cenv', env') <- check_specs mn [] [] specs;
+(check_signature mn init_decls decls cenv env NONE = 
+  return (decls, cenv, env)) ∧
+(check_signature mn init_decls decls cenv env (SOME specs) =
+  do (decls', cenv', env') <- check_specs mn ([],[],[]) [] [] specs;
      () <- guard (check_flat_weakC cenv cenv') "Signature mismatch";
      () <- check_weakE env env';
-     return (cenv',env')
+     () <- guard (check_weak_decls decls decls') "Signature mismatch";
+     return (decls',cenv',env')
   od)`;
 
 val infer_top_def = Define `
-(infer_top tdecs menv cenv env (Tdec d) =
+(infer_top decls menv cenv env (Tdec d) =
   do
-    (tdecs',cenv',env') <- infer_d NONE tdecs menv cenv env d;
-    return (tdecs',emp, (emp,cenv'), env')
+    (decls',cenv',env') <- infer_d NONE decls menv cenv env d;
+    return (decls',emp, (emp,cenv'), env')
   od) ∧
-(infer_top tdecs menv cenv env (Tmod mn spec ds1) =
+(infer_top (mdecls,tdecls,edecls) menv cenv env (Tmod mn spec ds1) =
   do
-    () <- guard (~MEM mn (MAP FST menv)) ("Duplicate module: " ++ mn);
-    (tdecs',cenv',env') <- infer_ds (SOME mn) tdecs menv cenv env ds1;
-    (cenv'',env'') <- check_signature (SOME mn) cenv' env' spec;
-    return (tdecs',[(mn,env'')], ([(mn,cenv'')],emp), emp)
+    () <- guard (~MEM mn mdecls) ("Duplicate module: " ++ mn);
+    (decls',cenv',env') <- infer_ds (SOME mn) (mdecls,tdecls,edecls) menv cenv env ds1;
+    ((mdecls'',tdecls'',edecls''),cenv'',env'') <- check_signature (SOME mn) (mdecls,tdecls,edecls) decls' cenv' env' spec;
+    return ((mn::mdecls'',tdecls'',edecls''),[(mn,env'')], ([(mn,cenv'')],emp), emp)
   od)`;
 
 val infer_prog_def = Define `
-(infer_prog menv cenv env [] =
-  return ([],([],[]),[])) ∧
-(infer_prog menv cenv env (top::ds) =
+(infer_prog decls menv cenv env [] =
+  return (([],[],[]),[],([],[]),[])) ∧
+(infer_prog decls menv cenv env (top::ds) =
   do
-    (menv',cenv',env') <- infer_top menv cenv env top;
-    (menv'', cenv'', env'') <- infer_prog menv (merge_tenvC cenv' cenv) (env' ++ env) ds;
-    return (menv''++menv', merge_tenvC cenv'' cenv', env'' ++ env')
+    (decls',menv',cenv',env') <- infer_top decls menv cenv env top;
+    (decls'', menv'', cenv'', env'') <- infer_prog (append_decls decls' decls) menv (merge_tenvC cenv' cenv) (env' ++ env) ds;
+    return (append_decls decls'' decls', menv''++menv', merge_tenvC cenv'' cenv', env'' ++ env')
   od)`;
 
 val Infer_Tfn_def = Define `
